Gadgets.v
@@ -1,7 +1,6 @@
 Require Import Metalib.Metatheory.
 Require Import Bool.
 From STLCZK Require Import GaloisField.
-From STLCZK Require Import Stlc.
 From STLCZK Require Import R1cs.
 From STLCZK Require Import Ltac.
 
@@ -19,74 +18,10 @@ Generalizable All Variables.
 Module Gadget(PF: GaloisField).
   Import PF.
   Include R1CS PF.
-  Include Stlc PF.
+
   Import MonadNotation.
   Open Scope monad_scope.
   Open Scope nat_scope.
-  
-  (** TR closure *)
-  Inductive multi {X : Type} (R : relation X) : relation X :=
-  | multi_refl : forall (x : X), multi R x x
-  | multi_step : forall (x y z : X),
-      R x y ->
-      multi R y z ->
-      multi R x z.
-  Notation " t '-->*' t' " := (multi step t t') (at level 40).
-
-  (** TRC with step count *)
-  Inductive multi_k {X: Type} (R: relation X) : nat -> relation X :=
-  | multi_k_refl: forall e,
-      multi_k R 0 e e
-  | multi_k_trans: forall a b c n,
-      R a b ->
-      multi_k R n b c ->
-      multi_k R (S n) a c.
-  Notation " t '==>*' k t' " := (multi_k step k t t') (at level 40).
-
-  Definition circuit_equiv(c: exp) (c': exp): Prop :=
-    forall (n: Fp), forall (w: Fp),
-        (<{ c' (fp n) (fp w) }> -->* <{ true }> <->
-        <{ c (fp n) }> -->* <{ fp w }>). 
-  Notation "a '~~' b" := (circuit_equiv a b) (at level 50).
-
-  Fixpoint normalize(e: exp) :=
-    match e with
-    | tm_app (tm_abs T e1) v1 =>
-      open_exp_wrt_exp (normalize e1) (normalize v1)
-    | tm_abs T e => tm_abs T e
-    | tm_app e1 e2 => tm_app (normalize e1) (normalize e2)
-    | tm_let e1 e2 =>
-      open_exp_wrt_exp (normalize e2) (normalize e1)
-    | tm_binop a op b =>
-      tm_binop (normalize a) op (normalize b)
-    | tm_eq e1 e2 =>
-      tm_eq (normalize e1) (normalize e2)
-    | tm_not e1 => tm_not (normalize e1)
-    | tm_ifthenelse e e1 e2 =>
-      tm_ifthenelse (normalize e) (normalize e1) (normalize e2)
-    | e => e
-    end.
-
-  Fixpoint normalizer(e: exp)(gas: nat): exp :=
-    match gas with
-    | 0%nat => e
-    | S g' => normalizer (normalize e) g'
-    end.
-
-  Definition normalization_lemma: forall e e', (exists G, normalizer e G = e') <-> e -->* e'.
-  Admitted.  
-
-  Inductive fo_type: typ -> Prop :=
-  | fot_fp:  fo_type <{{ Field }}> 
-  | fot_bool: fo_type <{{ Bool }}>.
- 
-  Inductive fo_value: exp -> typ -> Fp -> Prop :=
-  | fos_fp: forall p, fo_value <{ fp p }> <{{ Field }}> p
-  | fos_true: fo_value <{ true }> <{{ Bool }}> (1:%p)
-  | fos_false: fo_value <{ false }> <{{ Bool }}> (0:%p).
-
-  Import ListNotations.
-  Local Open Scope list_scope.
 
   Inductive r1cs_equiv: forall i v, exp -> @r1cs i v -> Prop :=
   | BaseTrue: forall e v (r: @r1cs 0 v) (vars: Vfp v),
